share/pulse/examples/dice/cbor/COSE.AST.fst
@@ -5,21 +5,60 @@ module Spec = COSE.Spec
 #push-options "--fuel 0"
 
 [@@  sem_attr]
-let e0 = empty_wf_ast_env
+let e0 = empty_total_env
 
 [@@  sem_attr]
 let generic_headers: group NMapGroup =
   GZeroOrOne (GMapElem () false (TElem (ELiteral (LInt CBOR.Spec.Constants.cbor_major_type_uint64 Spec.h_alg))) tint)
 
-[@@  sem_attr]
-let header_map = TMap generic_headers
+// expected: `option (either U64.t U64.t & ... )`
 
-let e1 = wf_ast_env_extend_typ
+
+
+[@@  sem_attr]
+let header_map = rewrite_typ 42 (TMap generic_headers) // TODO: embed this "rewrite" in the environment extension
+
+let header_map_wf = // PLEASE normalize this
+  compute_wf_typ
+    e0.te_ast.ta_ast
+    "header_map"
+    (_ by (FStar.Tactics.tadmit ()))
+    header_map
+    (_ by (FStar.Tactics.tadmit ())) // solve_mk_wf_typ_fuel_for ()))
+
+inline_for_extraction noextract
+let e1 = total_env_extend_typ
   e0
   "header_map"
-  (_ by (solve_by_norm ()))
-  header_map
-  (_ by (solve_mk_wf_typ_fuel_for ()))
+  header_map_wf
+  high_typ
+  high_typ_bij
+  low_typ
+  low_typ_bij
+
+let header_map_validator = e1.te_impl_validate "header_map" //PLEASE normalize
+let header_map_parser = e1.te_impl_parse "header_map" //PLEASE normalize
+let header_map_serializer = e1.te_impl_serialize "header_map" //PLEASE normalize
+
+inline_for_extraction noextract
+let e2 = total_env_replace
+  e1
+  "header_map"
+  header_map_validator
+  header_map_parser
+  header_map_serializer
+
+
+(*
+1 => string
+2 => int
+* (int => any)
+*)
+
+
+let header_map_wf = e0.te_impl_validate
+
+l
 
 irreducible let print (#t: Type) (x: t) : prop = False
 
